equation for exprD (App case) syntactic unificaiton problems
- A little bit of work on Subst including an
  ordering defined based on logical implication.
- unfolding equation for the application case of
  [exprD]
- PROBLEM: The naive formulation of [exprUnify]
  doesn't work any more because applications are not
  canonical. It seems like a good solution to this
  is to make [App] canonical, so that it takes a single
  argument. This acutally makes the representation more
  efficient and avoids a lot of annoying definitions of
  structural recursion.
  - Its only drawbacks seem to be places where you make
    bad assumptions.

src/Ext/ExprUnifySyntactic.v
@@ -1,51 +1,56 @@
 Require Import List.
-Require Import Expr.
-Require Import ExprUnify.
-Require Import Subst.
-Require Import Prover.
+Require Import MirrorCore.Prover.
+Require Import MirrorCore.Subst.
+Require Import MirrorCore.Ext.ExprCore.
+Require Import MirrorCore.Ext.ExprLift.
 
 Set Implicit Arguments.
 Set Strict Implicit.
 
 Section typed.
-  Variable ts : types.
   Variable subst : Type.
-  Variable Subst_subst : Subst ts subst. 
-  Variable p : ProverT ts.
-  Variable f : Facts p.
-  
-  Variable exprUnify : forall (n : nat) (s : subst) (l r : expr ts), option subst.
+  Variable types : Types.types.
+  Variable funcs : functions types.
+  Variable Subst_subst : Subst subst expr.
+  Variable SubstOk_subst : SubstOk (Expr_expr funcs) Subst_subst.
 
-  Fixpoint exprUnify' (n : nat) (s : subst) (e1 e2 : expr ts) {struct e1} : option subst.
+  Section nested.
+    (** n is the number of binders that we have gone under **)
+  Variable exprUnify : forall (under : nat) (s : subst) (l r : expr), option subst.
+
+  (** TODO: This algorithm is very weak, in particular it breaks down
+   ** because functions are first-class which means that there are multiple
+   ** representations of [f x y], e.g.
+   **   (((f nil) (a :: nil)) (b :: nil)),
+   **   (f (a :: b :: nil))
+   **   etc.
+   **)
+  Fixpoint exprUnify' (n : nat) (s : subst) (e1 e2 : expr) {struct e1}
+  : option subst.
   refine (
     match e1 , e2 with
-      | Const t1 v1 , Const t2 v2 =>
-        match const_seqb ts _ t1 t2 v1 v2 with
-          | Some true => Some s
-          | _ => None
-        end
-      | UVar u1 , UVar u2 => 
+      | UVar u1 , UVar u2 =>
         if EqNat.beq_nat u1 u2 then Some s
-          else
-            match Subst.set _ _ u1 (UVar u2) s with
-              | None => Subst.set _ _ u2 (UVar u1) s
-              | x => x
-            end
-      | UVar u1 , _ => 
-        match Subst.lookup _ _ u1 s with
-          | None => 
+        else
+          match Subst.set u1 (UVar u2) s with
+            | None => Subst.set u2 (UVar u1) s
+            | x => x
+          end
+      | UVar u1 , _ =>
+        match Subst.lookup u1 s with
+          | None =>
             match lower n n e2 with
               | None => None
-              | Some e2 => Subst.set _ _ u1 e2 s
+              | Some e2 => Subst.set u1 e2 s
             end
           | Some e1' => exprUnify n s e1' e2
         end
-      | _ , UVar u2 => 
-        match Subst.lookup _ _ u2 s with
+      | _ , UVar u2 =>
+        match Subst.lookup  u2 s with
           | None =>
             match lower n n e1 with
               | None => None
-              | Some e2 => Subst.set _ _ u2 e1 s
+              | Some e2 => Subst.set u2 e1 s
             end
           | Some e2' => exprUnify n s e1 e2'
         end
@@ -54,10 +59,15 @@ Section typed.
       | Func f1 ts1 , Func f2 fs2 =>
         if EqNat.beq_nat f1 f2 then Some s else None
       | App e1 es1 , App e2 es2 =>
+        (** TODO: This case is not correct, it is drastically simplified by
+         ** having a canonical representation of application for example:
+         **   [App e1 e2]  rather than [App e es]
+         **)
         match exprUnify' n s e1 e2 with
           | None => None
           | Some s' =>
-            (fix unifyArgs (s : subst) (es1 es2 : exprs ts) {struct es1} : option subst :=
+            (fix unifyArgs (s : subst) (es1 es2 : list expr) {struct es1}
+             : option subst :=
               match es1 , es2 with
                 | nil , nil => Some s
                 | e1 :: es1 , e2 :: es2 =>
@@ -71,9 +81,72 @@ Section typed.
       | Abs t1 e1 , Abs t2 e2 =>
         (* t1 = t2 since both terms have the same type *)
         exprUnify' (S n) s e1 e2
-      | _ , _ => None 
+      | _ , _ => None
     end).
   Defined.
+  End nested.
+
+  Fixpoint exprUnify (fuel : nat) (under : nat) (s : subst) (e1 e2 : expr)
+  : option subst :=
+    match fuel with
+      | 0 => None
+      | S fuel =>
+        exprUnify' (exprUnify fuel) under s e1 e2
+    end.
+
+  Require Import ExtLib.Tactics.Consider.
+  Require Import ExtLib.Tactics.Injection.
+
+  Definition unify_sound (unify : forall (under : nat) (s : subst) (l r : expr), option subst) : Prop := forall e1 e2 under s s' t u v,
+    exprD funcs u v e1 t <> None ->
+    exprD funcs u v e2 t <> None ->
+    unify under s e1 e2 = Some s' ->
+    substD (SubstOk := SubstOk_subst) u v s' ->
+       exprD funcs u v e1 t = exprD funcs u v e2 t
+    /\ substD (SubstOk := SubstOk_subst) u v s.
+
+  Lemma exprUnify'_sound : forall unify,
+                             unify_sound unify ->
+                             unify_sound (exprUnify' unify).
+  Proof.
+    red. induction e1; simpl; intros.
+    { destruct e2; try congruence.
+      { consider (EqNat.beq_nat v v1); intros; try congruence. subst.
+        inv_all; subst. intuition. }
+      { admit. } }
+    { destruct e2; try congruence.
+      { consider (EqNat.beq_nat f f0); try congruence; intros; subst.
+        inv_all; subst. split; auto.
+        admit. }
+      { admit. } }
+    { admit. }
+    { destruct e2; try congruence.
+      { consider (exprUnify' unify under s e1 e2); try congruence; intros.
+        { consider (typeof funcs u (map (@projT1 _ _) v) e1); intros.
+          specialize (IHe1 e2 under s s0 t0 u v).
+          repeat rewrite exprD_App in *.
+          repeat match goal with
+                   | |- _ => progress (inv_all; subst)
+                   | [ _ : not (match ?X with _ => _ end = None) |- _ ] =>
+                     (consider X; try congruence); [ intros ]
+                 end.
+
+  Admitted.
+
+  Theorem exprUnify_sound : forall fuel, unify_sound (exprUnify fuel).
+  Proof.
+    induction fuel; simpl; intros; try congruence.
+    eapply exprUnify'_sound. eassumption.
+  Qed.
+
+  Theorem exprUnify_var : forall fuel under s v e2,
+    exprUnify fuel under s (Var v) e2 =
+    match e2 with
+      | Var v' => None
+      | _ => None
+    end.
+  Abort.
+
 End typed.
 
 (*
@@ -82,7 +155,7 @@ End typed.
   refine (fun Subst Subst_Subst Prover Facts =>
     (** TODO: Use the prover in places where I return [None] **)
     (fix exprUnify (n : nat) : Subst -> expr ts -> expr ts -> option Subst :=
-      match n with 
+      match n with
         | 0 => fun _ _ _ => None
         | S n =>
           (fix unify s (e1 e2 : expr ts) {struct e1} : option Subst :=
@@ -92,19 +165,19 @@ End typed.
                   | Some true => Some s
                   | _ => None
                 end
-              | UVar u1 , UVar u2 => 
+              | UVar u1 , UVar u2 =>
                 if EqNat.beq_nat u1 u2 then Some s
                 else
                   match Subst.set _ _ u1 (UVar u2) s with
                     | None => Subst.set _ _ u2 (UVar u1) s
                     | x => x
                   end
-              | UVar u1 , _ => 
+              | UVar u1 , _ =>
                 match Subst.lookup _ _ u1 s with
                   | None => Subst.set _ _ u1 e2 s
                   | Some e1' => exprUnify n s e1' e2
                 end
-              | _ , UVar u2 => 
+              | _ , UVar u2 =>
                 match Subst.lookup _ _ u2 s with
                   | None => Subst.set _ _ u2 e1 s
                   | Some e2' => exprUnify n s e1 e2'
@@ -136,7 +209,7 @@ End typed.
                  ** because the ?1 isn't going to have x in scope
                  **)
                 unify s e1 e2
-              | _ , _ => None 
+              | _ , _ => None
             end)
       end) 10).
   Defined.
