src/ExprUnify.v
@@ -5,11 +5,18 @@ Require Import Prover.
 Set Implicit Arguments.
 Set Strict Implicit.
 
-Definition unifier  (ts : types) : Type :=
-  forall (S : Type) (Subst_S : Subst ts S) (P : ProverT ts),
-    Facts P ->
-    S -> expr ts -> expr ts -> option S.
+Section typed.
+  Variables typ expr uvar : Type.
 
+  Variable typD : list Type -> typ -> Type.
+  Context {Expr_expr : @Expr typ typD expr}.
+
+  Definition unifier : Type :=
+    forall (S : Type) (Subst_S : Subst S expr uvar) (P : @ProverT typ expr),
+      Facts P ->
+      S -> expr -> expr -> option S.
+
+(*
 Definition unifier_WellTyped (ts : types) (fs : tfunctions) (unify : unifier ts) : Prop :=
   forall  (S : Type) (Subst_S : Subst ts S) (P : ProverT ts)
     (F : Facts P) (subst : S) (e1 e2 : expr ts) subst',
@@ -22,7 +29,12 @@ Definition unifier_WellTyped (ts : types) (fs : tfunctions) (unify : unifier ts)
       WellTyped_Subst fs uenv venv subst'.
 *)
       True.
+*)
 
-Definition unifier_sound (ts : types) (fs : functions ts) (unify : unifier ts) : Prop :=
-  forall (S : Type) (Subst_S : Subst ts S) (P : ProverT ts) (PC : ProverT_correct P fs) (F : Facts P) (subst : S) (e1 e2 : expr ts) subst',
-    unify _ _ P F subst e1 e2 = Some subst' -> True.
+  Definition unifier_sound (unify : unifier) : Prop :=
+    forall (S : Type) (Subst_S : Subst S expr uvar)
+           (P : ProverT expr) (*PC : ProverT_correct P fs*)
+           (F : Facts P) (subst : S) (e1 e2 : expr) subst',
+      unify _ _ P F subst e1 e2 = Some subst' ->
+      forall us vs t,
+        exprD us vs e1 t = exprD us vs e2 t.
