src/Ext/ExprCore.v
@@ -288,6 +288,379 @@ Section env.
       | Some f => Some (f vs)
     end.
 
+  Require Import ExtLib.Tactics.Injection.
+  Require Import ExtLib.Tactics.EqDep.
+  Require Import ExtLib.Data.ListNth.
+
+
+    Theorem split_env_nth_error : forall ve v tv,
+      nth_error ve v = Some tv <->
+      match nth_error (projT1 (split_env ve)) v as t
+      return match t with
+               | Some v => typD types nil v
+               | None => unit
+             end -> Prop
+      with
+        | None => fun _ => False
+        | Some v => fun res => tv = existT _ v res
+      end (hlist_nth (projT2 (split_env ve)) v).
+    Proof.
+      induction ve; simpl; intros.
+      { destruct v; simpl in *; intuition; inversion H. }
+      { destruct v; simpl in *.
+        { intuition.
+          { inversion H; subst. destruct tv; reflexivity. }
+          { subst. destruct a. reflexivity. } }
+        { eapply IHve. } }
+    Qed.
+
+  Theorem exprD_Var : forall ve v t,
+    exprD ve (Var v) t = lookupAs ve v t.
+  Proof.
+    unfold exprD; simpl; intros.
+    consider (split_env ve); intros.
+    unfold lookupAs.
+    generalize (split_env_nth_error ve v).
+    consider (nth_error ve v).
+    { intros. destruct (H1 s); clear H1. clear H3. specialize (H2 eq_refl).
+      rewrite H in *. simpl in *.
+      destruct s; simpl in *.
+      revert H2.
+      change (
+          let f' e0 := hlist_nth e0 v in
+          match
+            nth_error x v as t1
+            return
+            (match t1 with
+               | Some v0 => typD types nil v0
+               | None => unit
+             end -> Prop)
+          with
+            | Some v0 =>
+              fun res : typD types nil v0 =>
+                existT (typD types nil) x0 t0 = existT (typD types nil) v0 res
+            | None => fun _ : unit => False
+          end (f' h) ->
+          match
+            match
+              nth_error x v as z
+              return
+              (z = nth_error x v ->
+               option (hlist (typD types nil) x -> typD types nil t))
+            with
+              | Some t' =>
+                fun pf : Some t' = nth_error x v =>
+                  match typ_cast_typ types (fun x1 : Type => x1) nil t' t with
+                    | Some f =>
+                      Some
+                        (fun e0 : hlist (typD types nil) x =>
+                           match
+                             pf in (_ = t'')
+                             return
+                             (match t'' with
+                                | Some t1 => typD types nil t1
+                                | None => unit
+                              end -> typD types nil t)
+                           with
+                             | eq_refl => fun x1 : typD types nil t' => f x1
+                           end (f' e0))
+                    | None => None
+                  end
+              | None => fun _ : None = nth_error x v => None
+            end eq_refl
+          with
+            | Some f => Some (f h)
+            | None => None
+          end =
+          match typ_cast_typ types (fun x1 : Type => x1) nil x0 t with
+            | Some f => Some (f t0)
+            | None => None
+          end).
+      match goal with
+        | |- context [ @eq_refl ?X ?Y ] =>
+          generalize dependent (@eq_refl X Y)
+      end.
+      pattern (nth_error x v) at 1 5.
+      destruct (nth_error x v).
+      { intro.
+        assert (nth_error x v = Some x0).
+        { cutrewrite (x = projT1 (split_env ve)).
+          rewrite split_env_projT1.
+          erewrite map_nth_error. 2: eassumption. reflexivity.
+          rewrite H. reflexivity. }
+        { assert (x0 = t1).
+          { rewrite H1 in e. inv_all; auto. }
+          subst. destruct (typ_cast_typ types (fun x => x) nil t1 t); auto.
+          { intros. f_equal.
+            subst f'. simpl in *. generalize dependent (hlist_nth h v).
+            generalize dependent (nth_error x v).
+            intros; subst.
+            inv_all. f_equal; auto. } } }
+      { simpl. intro. generalize dependent (hlist_nth h v).
+        rewrite <- e. intuition. } }
+    { intro.
+      assert (nth_error x v = None).
+      { cutrewrite (x = projT1 (split_env ve)).
+        rewrite split_env_projT1.
+        rewrite nth_error_map.
+        rewrite H0. reflexivity.
+        rewrite H. reflexivity. }
+      { match goal with
+          | |- context [ @eq_refl ?X ?Y ] =>
+            generalize dependent (@eq_refl X Y)
+        end.
+        rewrite H; simpl. intros. clear H2.
+        change (
+            let f t' := fun pf : Some t' = nth_error x v =>
+                    match typ_cast_typ types (fun x0 : Type => x0) nil t' t with
+                      | Some f =>
+                        Some
+                          (fun e0 : hlist (typD types nil) x =>
+                             match
+                               pf in (_ = t'')
+                               return
+                               (match t'' with
+                                  | Some t0 => typD types nil t0
+                                  | None => unit
+                                end -> typD types nil t)
+                             with
+                               | eq_refl => fun x0 : typD types nil t' => f x0
+                             end (hlist_nth e0 v))
+                      | None => None
+                    end in
+            match
+              match
+                nth_error x v as z
+                return
+                (z = nth_error x v ->
+                 option (hlist (typD types nil) x -> typD types nil t))
+              with
+                | Some t' => f t'
+                | None => fun _ : None = nth_error x v => None
+              end e
+            with
+              | Some f => Some (f h)
+              | None => None
+            end = None
+          ).
+        intro. clearbody f.
+        revert e.
+        pattern (nth_error x v) at 1 3.
+        rewrite H1. reflexivity. } }
+  Qed.
+
+  Theorem exprD_UVar : forall ve u t,
+    exprD ve (UVar u) t = lookupAs meta_env u t.
+  Proof.
+    unfold exprD. intros.
+    destruct (split_env ve); simpl.
+    destruct (lookupAs meta_env u t); auto.
+  Qed.
+
+  Theorem exprD_Equal : forall ve t l r,
+    exprD ve (Equal t l r) tvProp =
+    match exprD ve l t , exprD ve r t with
+      | Some l , Some r => Some (l = r)
+      | _ , _ => None
+    end.
+  Proof.
+    unfold exprD; intros.
+    destruct (split_env ve); simpl.
+    destruct (exprD' x l t); destruct (exprD' x r t); auto.
+  Qed.
+
+  Theorem exprD_Not : forall ve p,
+    exprD ve (Not p) tvProp =
+    match exprD ve p tvProp with
+      | Some p => Some (~p)
+      | _ => None
+    end.
+  Proof.
+    unfold exprD; intros.
+    destruct (split_env ve); simpl.
+    destruct (exprD' x p tvProp); auto.
+  Qed.
+
+  Fixpoint arrow (ls : list typ) (r : typ) : typ :=
+    match ls with
+      | nil => r
+      | l :: ls => tvArr l (arrow ls r)
+    end.
+
+  Fixpoint apply {ts} {ls : list typ} {r : typ} (f : typD types ts (arrow ls r))
+           (args : hlist (typD types ts) ls) : typD types ts r :=
+    match args in hlist _ ls
+          return typD types ts (arrow ls r) -> typD types ts r
+    with
+      | Hnil => fun x => x
+      | Hcons _ _ v vs => fun x => apply (x v) vs
+    end f.
+
+  Fixpoint mapD {T : Type} {F : T -> Type} (f : forall x, F x) (ls : list T)
+  : hlist F ls :=
+    match ls with
+      | nil => Hnil
+      | l :: ls => @Hcons T F l ls (f l) (mapD f ls)
+    end.
+
+  Fixpoint mapD2 {T U : Type} {F : T -> Type} (f : U -> forall x, F x) (ls : list (U * T))
+  : hlist F (map snd ls) :=
+    match ls as ls return hlist F (map snd ls) with
+      | nil => Hnil
+      | (l,l') :: ls => @Hcons T F _ _ (f l l') (mapD2 f ls)
+    end.
+
+  Theorem exprD_Abs : forall ve t u e val,
+    exprD ve (Abs t e) (tvArr t u) = Some val ->
+    forall x, exprD (existT _ t x :: ve) e u = Some (val x).
+  Proof.
+    unfold exprD. intros.
+    change (split_env (existT (typD types nil) t x :: ve))
+      with (split_env ((existT (typD types nil) t x :: nil) ++ ve)).
+    rewrite split_env_app.
+    destruct (split_env ve). simpl in *.
+    rewrite typ_cast_typ_refl in *.
+    destruct (exprD' (t :: x0) e u); intuition (try congruence).
+    inv_all; subst. reflexivity.
+  Qed.
+
+  Theorem typ_cast_typ_eq : forall f ts t t' v,
+                              typ_cast_typ types f ts t t' = Some v -> t = t'.
+  Proof.
+    clear. unfold typ_cast_typ; simpl; intros.
+    destruct (typ_eq_odec t t'); auto. congruence.
+  Qed.
+
+  Theorem exprD'_typeof : forall e ve t v,
+    exprD' ve e t = Some v ->
+    typeof ve e = Some t.
+  Proof.
+    induction e; simpl; intros; auto;
+    repeat match goal with
+             | [ H : context [ match ?X with _ => _ end ] |- _ ] =>
+               (consider X; intros; try congruence); [ inv_all; subst ]
+           end.
+    { match type of H with
+        | _ ?X = _ => generalize dependent X
+      end.
+      pattern (nth_error ve v) at 1 3.
+      destruct (nth_error ve v); try congruence.
+      intros.
+      match goal with
+        | [ H : context [ match ?X with _ => _ end ] |- _ ] =>
+          (consider X; intros; try congruence); [ inv_all; subst ]
+      end.
+      unfold typ_cast_typ in H.
+      rewrite <- e.
+      destruct (typ_eq_odec t0 t); subst; auto. congruence. }
+    { destruct f0; simpl in *. clear H. f_equal.
+      generalize dependent ftype0.
+      induction ts; simpl; intros.
+      { destruct fenv0; simpl in *. inv_all; subst.
+        Lemma typ_cast_val_eq : forall ts a b v v', 
+                                  typ_cast_val ts a b v = Some v' ->
+                                  a = b.
+        Proof.
+          clear. unfold typ_cast_val; simpl; intros.
+          unfold typ_cast_typ in *. generalize (@typ_eq_odec_None a b).
+          destruct (typ_eq_odec a b); auto. congruence.
+        Qed.
+        eapply typ_cast_val_eq in H1. auto. congruence. }
+      { destruct fenv0; simpl in *; try congruence.
+        match goal with
+          | H : match ?X with _ => _ end = _ |- _ =>
+            consider X
+        end; intros; try congruence.
+        inv_all; subst.
+        specialize (IHts _ fdenote0). unfold typ_cast_val in *.
+        unfold typ_cast_typ in *.
+        generalize (@typ_eq_odec_None (subst0_typ a (instantiate_typ ts ftype0)) t).
+        destruct (typ_eq_odec (subst0_typ a (instantiate_typ ts ftype0)) t); try congruence. } }
+    { unfold lookupAs in *.
+      destruct (nth_error meta_env v).
+      { destruct s. simpl in *.
+        unfold typ_cast_typ in *.
+        destruct (typ_eq_odec x t); subst; auto.
+        congruence. }
+      { congruence. } }
+    { clear H1 H0 IHe. generalize dependent t0. generalize dependent t. clear - H.
+      induction H; simpl; intros.
+      { generalize (@typ_cast_typ_eq (fun x => x) nil t0 t).
+        destruct (typ_cast_typ types (fun x : Type => x) nil t0 t); try congruence.
+        inv_all. subst. intros. specialize (H _ eq_refl). subst; auto. }
+      { destruct t0; try congruence.
+        consider (exprD' ve x t0_1); try congruence; intros. eapply H in H1.
+        rewrite H1 in *. simpl in *.
+        change (typ_eqb t0_1 t0_1) with (t0_1 ?[ eq ] t0_1).
+        consider (t0_1 ?[ eq ] t0_1); try congruence; intros.
+        clear H3. eapply IHForall; eauto. } }
+    { eapply IHe in H0.
+      generalize (typ_cast_typ_eq (fun x => x) nil t1 t H); intros; subst.
+      rewrite H0. reflexivity. }
+    { destruct t0; auto; congruence. }
+    { destruct t; auto; congruence. }
+  Qed.
+
+  Theorem exprD_app_nil : forall ve t e,
+    exprD ve (App e nil) t = exprD ve e t.
+  Proof.
+    unfold exprD; simpl; intros.
+    destruct (split_env ve); simpl in *.
+    consider (exprD' x e t); intros.
+    { rewrite (exprD'_typeof _ _ H).
+      rewrite H.
+      rewrite typ_cast_typ_refl. reflexivity. }
+    { consider (typeof x e); intros; auto.
+      { unfold typ_cast_typ.
+        destruct (typ_eq_odec t0 t); subst.
+        { rewrite H. reflexivity. }
+        { destruct (exprD' x e t0); auto. } } }
+  Qed.
+
+  Theorem exprD_App : forall ve t e args,
+    exprD ve (App e args) t =
+    match typeof (map (@projT1 _ _) ve) e with
+      | None => None
+      | Some tf =>
+        match exprD ve e tf with
+          | None => None
+          | Some f =>
+            (fix eval_args (tf : typ) (f : typD types nil tf) (args : list expr)
+                 {struct args}
+             : option (typD types nil t) :=
+               match args with
+                 | nil => typ_cast_val nil tf t f
+                 | arg :: args =>
+                   match tf as tf
+                         return typD types nil tf -> option (typD types nil t)
+                   with
+                     | tvArr l r => fun f =>
+                       match exprD ve arg l with
+                         | None => None
+                         | Some argv =>
+                           eval_args r (f argv) args
+                       end
+                     | _ => fun _ => None
+                   end f
+               end) tf f args
+        end
+    end.
+  Proof.
+    intros; simpl.
+    unfold exprD; simpl; intros.
+    rewrite <- split_env_projT1.
+    destruct (split_env ve); simpl in *; intros.
+    destruct (typeof x e); auto.
+    destruct (exprD' x e t0); auto.
+    clear. generalize dependent t0.
+    induction args; simpl; intros.
+    { unfold typ_cast_val.
+      destruct (typ_cast_typ types (fun x0 : Type => x0) nil t0 t); auto. }
+    { destruct t0; auto.
+      destruct (exprD' x a t0_1); auto.
+      rewrite IHargs. reflexivity. }
+  Qed.
+
   Fixpoint anyb {T} (p : T -> bool) (ls : list T) : bool :=
     match ls with
       | nil => false
@@ -310,15 +683,6 @@ Section env.
       | Equal _ e1 e2 => if mentionsU u e1 then true else mentionsU u e2
       | Not e => mentionsU u e
     end.
-
-(*
-  Definition const_seqb ts (a b : typ) (x : typD types ts a) (y : typD types ts b)
-  : option bool :=
-    match @typ_cast_val ts a b x with
-      | None => None
-      | Some x' => eqb ts b x' y
-    end.
-*)
 
   Fixpoint expr_eq_dec (e1 e2 : expr) : bool.
   refine (
