src/Subst.v
@@ -1,16 +1,63 @@
 Require Import List.
 Require Import Relations.
-Require Import Expr.
+
+Require Import MirrorCore.TypesI.
+Require Import MirrorCore.ExprI.
+
+Set Implicit Arguments.
+Set Strict Implicit.
 
 Section subst.
-  Variable ts : types.
   Variable T : Type.
+  Variable expr : Type.
+  Let uvar : Type := nat.
 
   Class Subst :=
-  { set : uvar -> expr ts -> T -> option T
-  ; lookup : uvar -> T -> option (expr ts)
+  { set : uvar -> expr -> T -> option T
+  ; lookup : uvar -> T -> option expr
+  ; subst : T -> expr -> expr
   }.
 
+  Variable typ : Type.
+  Variable typD : list Type -> typ -> Type.
+  Variable Expr_expr : Expr typD expr.
+
+  Class SubstOk (S : Subst) : Type :=
+  { substD : EnvI.env typD -> EnvI.env typD -> T -> Prop
+  ; substD_subst : forall u v s e t,
+                     substD u v s ->
+                     exprD u v e t = exprD u v (subst s e) t
+  ; substD_lookup : forall u v s uv e,
+                      lookup uv s = Some e ->
+                      substD u v s ->
+                      exists val, nth_error u uv = Some val /\
+                                  exprD u v e (projT1 val) = Some (projT2 val)
+  ; substD_set : forall s s' uv e,
+                   set uv e s = Some s' ->
+                   forall u v val,
+                     (substD u v s /\
+                      nth_error u uv = Some val /\
+                      exprD u v e (projT1 val) = Some (projT2 val)) <->
+                     (substD u v s')
+  }.
+
+  Variable Subst_subst : Subst.
+  Variable SubstOk_subst : SubstOk Subst_subst.
+
+  Definition Subst_Extends (a b : T) : Prop :=
+    forall u v, substD u v b -> substD u v a.
+
+  (** the [expr] type requires a notion of unification variable **)
+
+(*
+  Class SubstOk :=
+  { Subst_WellTyped : tfunctions -> tenv -> tenv -> T -> Prop
+  ; Subst_Extends : relation T
+  ; PreOrder_Subst_Extends : PreOrder Subst_Extends
+  }.
+*)
+
+(*
   Section instantiate.
     Variable Subst_T : Subst.
 
@@ -32,14 +79,10 @@ Section subst.
         | Not e => Not (exprInstantiate l e)
       end.
   End instantiate.
+*)
 
 (*
 
-  Class SubstOk :=
-  { Subst_WellTyped : tfunctions -> tenv -> tenv -> T -> Prop
-  ; Subst_Extends : relation T
-  ; PreOrder_Subst_Extends : PreOrder Subst_Extends
-  }.
 
 Section map_subst.
   Variable m : Type -> Type.
